gwhrnbgw

Games/games/Chomp_work.lean
@@ -103,6 +103,47 @@ structure Chomp_law (ini : Finset (ℕ × ℕ)) (hist : List (ℕ × ℕ)) (act 
   nd : ∀ q ∈ hist, nondomi q act
   nz_act : act ≠ (0,0)
 
+@[mk_iff]
+structure partiality_condition (ini : Finset (ℕ × ℕ)) (hist : List (ℕ × ℕ)) : Prop where
+  zero_ini : (0,0) ∈ ini
+  zero_hist : (0,0) ∉ hist
+  hist_ini : ∀ a ∈ hist, a ∈ ini
+  --state : Chomp_state ini hist ≠ {(0,0)}
+
+
+instance (ini : Finset (ℕ × ℕ)) (hist : List (ℕ × ℕ)) : Decidable (partiality_condition ini hist) :=
+  by
+  rw [partiality_condition_iff]
+  exact And.decidable
+
+--#exit
+
+-- instance (ini : Finset (ℕ × ℕ)) (hist : List (ℕ × ℕ)) : Decidable (partiality_condition ini hist) :=
+--   by
+--   have one : Decidable ((0,0) ∈ ini) := by exact Finset.decidableMem (0, 0) ini
+--   have two : Decidable ((0,0) ∉ hist) := by exact Not.decidable
+--   have three : Decidable (∀ a ∈ hist, a ∈ ini) := by exact List.decidableBAll (fun x => x ∈ ini) hist
+--   have four : Decidable (Chomp_state ini hist ≠ {(0,0)}) := by exact Not.decidable
+--   cases' one with one one
+--   · apply Decidable.isFalse
+--     intro con
+--     exact one con.zero_ini
+--   · cases' two with two two
+--     · apply Decidable.isFalse
+--       intro con
+--       exact two con.zero_hist
+--     · cases' three with three three
+--       · apply Decidable.isFalse
+--         intro con
+--         exact three con.hist_ini
+--       · cases' four with four four
+--         · apply Decidable.isFalse
+--           intro con
+--           exact four con.state
+--         · apply Decidable.isTrue
+--           exact ⟨one, two,three, four⟩
+
+
 
 def preChomp (height length : ℕ) : Symm_Game_World (Finset (ℕ × ℕ)) (ℕ × ℕ) where
   init_game_state := Chomp_init height length
@@ -110,14 +151,15 @@ def preChomp (height length : ℕ) : Symm_Game_World (Finset (ℕ × ℕ)) (ℕ 
   transition := fun ini hist act => if Chomp_state ini hist ≠ {(0,0)}
                                     then (Chomp_state ini) (act :: hist)
                                     else {(0,0)}
-  law := fun ini hist act => if (0,0) ∈ ini ∧ (0,0) ∉ hist
-                             then
+  law := fun ini hist act => if partiality_condition ini hist
+                             then -- fix ↑ ↓ and maybe instead reques Hist_legal wrt. Chomp_law ?
                               if Chomp_state ini hist ≠ {(0,0)}
                               then Chomp_law ini hist act
-                              else act ≠ (0,0) -- saves ass in `preChomp_law_careless`
+                              else act ≠ (0,0) ∧ act ∈ Chomp_state ini hist -- saves ass in `preChomp_law_careless`
                              else True
 
 
+--#exit
 
 lemma Chomp_state_ini_zero (hist : List (ℕ × ℕ)) (hh : (0,0) ∉ hist): Chomp_state {(0,0)} hist = {(0,0)} :=
   by
@@ -186,7 +228,6 @@ lemma Chomp_state_state_empty (ini : Finset (ℕ × ℕ) ) (hini : (0,0) ∈ ini
   convert qh <;> {rw [eq_comm] ; assumption}
 
 
-
 lemma Chomp_law_state_mem (ini : Finset (ℕ × ℕ) ) (hist : List (ℕ × ℕ)) (act : ℕ × ℕ) (leg : Chomp_law ini hist act) :
   act ∈ Chomp_state ini hist :=
   by
@@ -206,37 +247,70 @@ lemma Chomp_law_sub (ini : Finset (ℕ × ℕ) ) (l L : List (ℕ × ℕ)) (act 
   exact List.mem_append_right l qdef
 
 
+lemma Chomp_law_blind (ini : Finset (ℕ × ℕ) ) (l L : List (ℕ × ℕ)) (act : ℕ × ℕ) (leg : Chomp_law ini (l ++ L) act) :
+  Chomp_law (Chomp_state ini L) l act :=
+  by
+  refine' ⟨_ , _ , leg.nz_act⟩
+  · dsimp [Chomp_state]
+    rw [Finset.mem_filter]
+    refine' ⟨leg.act_mem, _⟩
+    intro q qdef
+    apply leg.nd
+    exact List.mem_append.mpr (Or.inr qdef)
+  · intro q qdef
+    apply leg.nd
+    exact List.mem_append.mpr (Or.inl qdef)
+
+
+
+
 
 lemma Chomp_hist_no_zero_of_Hist_legal (height length : ℕ) (ini : Finset (ℕ × ℕ) ) (hini : (0,0) ∈ ini) (prehist : List (ℕ × ℕ))
-  (main : Hist_legal (preChomp height length).law (preChomp height length).law ini prehist) : (0,0) ∉ prehist :=
+  (main : Hist_legal (preChomp height length).law (preChomp height length).law ini prehist) : (0,0) ∉ prehist ∧ (∀ a ∈ prehist, a ∈ ini) :=
   by
   induction' prehist with x l ih
-  · decide
+  · constructor
+    · decide
+    · intro a no ; contradiction
   · cases' main
     rename_i sofar now
-    apply List.not_mem_cons_of_ne_of_not_mem
-    · split_ifs at now
-      all_goals { dsimp [preChomp] at now
-                  rw [if_pos ⟨hini, ih sofar⟩ ] at now
-                  split_ifs at now
-                  · contrapose! now
-                    apply now.symm
-                  · rw [ne_comm]
-                    apply now.nz_act}
-    · exact ih sofar
+    constructor
+    · apply List.not_mem_cons_of_ne_of_not_mem
+      · split_ifs at now
+        all_goals { dsimp [preChomp] at now
+                    rw [if_pos ⟨hini, (ih sofar).1, (ih sofar).2⟩ ] at now
+                    split_ifs at now
+                    · intro con
+                      exact now.1 con.symm
+                    · rw [ne_comm]
+                      apply now.nz_act}
+      · exact (ih sofar).1
+    · intro a adef
+      rw [List.mem_cons] at adef
+      cases' adef with adef adef
+      · rw [adef]
+        split_ifs at now
+        all_goals { dsimp [preChomp] at now
+                    rw [if_pos ⟨hini, (ih sofar).1, (ih sofar).2⟩ ] at now
+                    split_ifs at now
+                    · exact (Chomp_state_sub_ini _ _) now.2
+                    · exact now.act_mem
 
+        }
+      · exact (ih sofar).2 a adef
 
+--#exit
 
 lemma preChomp_law_careless (height length : ℕ) :
   careless (preChomp height length).law (preChomp height length).law (preChomp height length).init_game_state (preChomp height length).law (preChomp height length).transition :=
   by
   intro ini hist prehist pHne pHl
   ext act
-  by_cases fix : (0,0) ∈ ini ∧ (0, 0) ∉ hist
+  by_cases fix : partiality_condition ini hist
   · constructor
     · intro c
       dsimp [preChomp] at c
-      rw [if_pos ⟨fix.1, (by apply List.not_mem_append fix.2 ; exact Chomp_hist_no_zero_of_Hist_legal height length ini fix.1 prehist pHl)⟩ ] at c
+      rw [if_pos ⟨fix.zero_ini, (by apply List.not_mem_append fix.zero_hist ; exact (Chomp_hist_no_zero_of_Hist_legal height length ini fix.zero_ini prehist pHl).1) , (by intro a adef ; rw [List.mem_append] at adef ; cases' adef with adef adef ; exact fix.hist_ini a adef ; exact (Chomp_hist_no_zero_of_Hist_legal height length ini fix.zero_ini prehist pHl).2 a adef)⟩ ] at c
       by_cases q1 : Chomp_state ini (hist ++ prehist) ≠ {(0,0)}
       · rw [if_pos q1] at c
         by_cases q2 : Chomp_state (Symm_Game_World.transition (preChomp height length) ini (List.tail prehist) (List.head prehist pHne)) (hist) ≠ {(0,0)}
@@ -279,7 +353,30 @@ lemma preChomp_law_careless (height length : ℕ) :
         · dsimp [preChomp] at *
           rw [if_neg q2]
           split_ifs
-          all_goals apply c.nz_act
+          · exfalso
+            rename_i nope no
+            replace no := no.hist_ini
+            cases' hist with x l
+            · have : Chomp_state ini ( prehist) = ∅ :=
+                by
+                rw [← @Finset.ssubset_singleton_iff _ _ (0,0), Finset.ssubset_iff_subset_ne]
+                constructor
+                · rw [← List.cons_head_tail _ pHne]
+                  rw [show List.head prehist pHne :: List.tail prehist = [List.head prehist pHne] ++ List.tail prehist from by rfl]
+                  rw [← nope]
+                  apply Chomp_state_sub'
+                · apply q1
+              replace this := Chomp_state_state_empty _ fix.zero_ini _ this
+              exact (Chomp_hist_no_zero_of_Hist_legal height length ini fix.zero_ini prehist pHl).1 this
+            · apply fix.zero_hist
+              specialize no x (by apply List.mem_cons_self)
+              rw [Finset.mem_singleton] at no
+              rw [← no]
+              apply List.mem_cons_self
+          · refine' ⟨c.nz_act, _ ⟩
+            apply Chomp_law_state_mem
+            rw [List.cons_head_tail _ pHne]
+            apply Chomp_law_blind _ _ _ _ c
       · rw [if_neg q1] at c
         by_cases q2 : Chomp_state (Symm_Game_World.transition (preChomp height length) ini (List.tail prehist) (List.head prehist pHne)) (hist) ≠ {(0,0)}
         · dsimp [preChomp] at *
@@ -318,10 +415,18 @@ lemma preChomp_law_careless (height length : ℕ) :
         · dsimp [preChomp] at *
           rw [if_neg q2]
           split_ifs
-          all_goals apply c
+          · rw [not_not] at q1
+            rw [q1] at c
+            rw [Chomp_state_ini_zero _ fix.zero_hist]
+            exact c
+          · rw [not_not] at q1 q2
+            rw [q1, Finset.mem_singleton] at c
+            exfalso
+            exact c.1 c.2
     · intro c
       dsimp [preChomp] at *
-      rw [if_pos ⟨fix.1, (by apply List.not_mem_append fix.2 ; exact Chomp_hist_no_zero_of_Hist_legal height length ini fix.1 prehist pHl)⟩ ]
+      rw [if_pos ⟨fix.zero_ini, (by apply List.not_mem_append fix.zero_hist ; exact (Chomp_hist_no_zero_of_Hist_legal height length ini fix.zero_ini prehist pHl).1) , (by intro a adef ; rw [List.mem_append] at adef ; cases' adef with adef adef ; exact fix.hist_ini a adef ; exact (Chomp_hist_no_zero_of_Hist_legal height length ini fix.zero_ini prehist pHl).2 a adef)⟩ ]
+      --rw [if_pos ⟨fix.1, (by apply List.not_mem_append fix.2 ; exact Chomp_hist_no_zero_of_Hist_legal height length ini fix.1 prehist pHl)⟩ ]
       rw [List.cons_head_tail] at *
       by_cases q1 : Chomp_state ini (hist ++ prehist) ≠ {(0,0)}
       · rw [if_pos q1]
@@ -434,7 +539,7 @@ lemma preChomp_law_careless (height length : ℕ) :
     · rename_i a b c
       exact False.elim (by apply fix ; constructor ; apply Chomp_state_sub_ini ; apply b.1 ; apply b.2)
 
-
+#exit
 
 
 lemma preChomp_tranistion_careless (height length : ℕ) :
@@ -875,52 +980,8 @@ lemma preChomp_law_prop_law (height length : ℕ) (h : height ≠ 0 ∨ length �
       · rw [if_neg q1] at leg
 
 
-lemma preChomp_law_prop_law' (height length : ℕ) (h : height ≠ 0 ∨ length ≠ 0) (act : ℕ × ℕ) (hist : List (ℕ × ℕ)) (hh : hist ≠ [])
-  (leg : Symm_Game_World.law (Chomp height length).toSymm_Game_World (Chomp height length).toSymm_Game_World.init_game_state hist act) :
-  Symm_Game_World.law (Chomp height length).toSymm_Game_World (Chomp height length).toSymm_Game_World.init_game_state
-  (hist ++ [(length, height)]) act :=
-  by
-  induction' hist with  x l ih
-  · contradiction
-  · dsimp [Chomp, preChomp] at *
-    by_cases q0 : (0, 0) ∉ x :: l
-    · rw [if_pos ⟨Chomp_init_has_zero height length, q0 ⟩ ] at leg
-      rw [if_pos _]
-      swap
-      · refine' ⟨Chomp_init_has_zero height length, _⟩
-        apply List.not_mem_append q0
-        intro con
-        rw [List.mem_singleton, Prod.eq_iff_fst_eq_snd_eq] at con
-        cases' h with h h
-        · exact False.elim (h con.2.symm)
-        · exact False.elim (h con.1.symm)
-      · by_cases q1 : ¬Chomp_state (Chomp_init height length) (x :: l) = {(0, 0)}
-        · rw [if_pos q1] at leg
-          by_cases q2 : ¬Chomp_state (Chomp_init height length) (x :: l ++ [(length, height)]) = {(0, 0)}
-          · rw [← List.cons_append, if_pos q2]
-            constructor
-            · exact leg.act_mem
-            · intro q qdef
-              rw [List.mem_append] at qdef
-              cases' qdef with qdef qdef
-              · exact leg.nd _ qdef
-              · rw [List.mem_singleton] at qdef
-                rw [qdef]
-                dsimp [nondomi, domi]
-                induction' hist with x hist ih
-                · contradiction
-                · have leg1 := leg.act_mem
-                  dsimp [Chomp_init] at leg1
-                  simp_rw [Finset.mem_product, Finset.mem_range, Nat.lt_add_one_iff] at leg1
-                  have leg2 := leg.nd x (List.mem_cons_self x hist)
 
-            · exact leg.nz_act
-          · rw [if_neg q2]
-            exact leg.nz_act
-        · rw [if_neg q1] at leg
-
-
-#exit
+--#exit
 
 lemma preChomp_law_prop (height length : ℕ) (h : height ≠ 0 ∨ length ≠ 0) : Strong_stealing_condition (Chomp height length ) :=
   by
